specs/tests/Spec.SHA3.Test.fst
@@ -23,10 +23,14 @@ let test_sha3 msg_len msg expected224 expected256 expected384 expected512 =
   let expected384:lbytes 48 = createL expected384 in
   let expected512:lbytes 64 = createL expected512 in
 
-  let test224 = Spec.SHA3.sha3_224 msg_len msg in
-  let test256 = Spec.SHA3.sha3_256 msg_len msg in
-  let test384 = Spec.SHA3.sha3_384 msg_len msg in
-  let test512 = Spec.SHA3.sha3_512 msg_len msg in
+  let test224 = create 28 (u8 0) in
+  let test224 = Spec.SHA3.sha3_224 msg_len msg test224 in
+  let test256 = create 32 (u8 0) in
+  let test256 = Spec.SHA3.sha3_256 msg_len msg test256 in
+  let test384 = create 48 (u8 0) in
+  let test384 = Spec.SHA3.sha3_384 msg_len msg test384 in
+  let test512 = create 64 (u8 0) in
+  let test512 = Spec.SHA3.sha3_512 msg_len msg test512 in
 
   let r224 = print_and_compare 28 expected224 test224 in
   let r256 = print_and_compare 32 expected256 test256 in
@@ -38,14 +42,16 @@ let test_shake128 msg_len msg out_len expected =
   let msg:lbytes msg_len = createL msg in
   let expected:lbytes out_len = createL expected in
 
-  let test = Spec.SHA3.shake128 msg_len msg out_len in
+  let test = create out_len (u8 0) in
+  let test = Spec.SHA3.shake128 msg_len msg out_len test in
   print_and_compare out_len expected test
 
 let test_shake256 msg_len msg out_len expected =
   let msg:lbytes msg_len = createL msg in
   let expected:lbytes out_len = createL expected in
 
-  let test = Spec.SHA3.shake256 msg_len msg out_len in
+  let test = create out_len (u8 0) in
+  let test = Spec.SHA3.shake256 msg_len msg out_len test in
   print_and_compare out_len expected test
 
 //
